Typing.thy
@@ -41,7 +41,9 @@ syntax
 translations
   "\<forall>x|\<in>|A. P" \<rightleftharpoons> "CONST fBall A (\<lambda>x. P)"
 
-inductive Tm :: "\<Gamma> \<Rightarrow> \<Delta> \<Rightarrow> term \<Rightarrow> \<tau> \<Rightarrow> bool" ("_ , _ \<turnstile> _ : _" 50) where
+inductive Tm :: "\<Gamma> \<Rightarrow> \<Delta> \<Rightarrow> term \<Rightarrow> \<tau> \<Rightarrow> bool" ("_ , _ \<turnstile> _ : _" 50) and
+          Alts :: "\<Gamma> \<Rightarrow> \<Delta> \<Rightarrow> term \<Rightarrow> alt_list \<Rightarrow> \<tau> \<Rightarrow> bool" and
+          Alt :: "\<Gamma> \<Rightarrow> \<Delta> \<Rightarrow> term \<Rightarrow> alt \<Rightarrow> \<tau> \<Rightarrow> bool" where
   Tm_Var: "\<lbrakk> \<Delta> \<turnstile> \<Gamma> ; BVar x \<tau> \<in> \<Gamma> \<rbrakk> \<Longrightarrow> \<Gamma> , \<Delta> \<turnstile> (Var x) : \<tau>"
 
 | Tm_Abs: "BVar x \<tau>1 # \<Gamma> , \<Delta> \<turnstile> e : \<tau>2 \<Longrightarrow> \<Gamma> , \<Delta> \<turnstile> (\<lambda> x : \<tau>1 . e) : (\<tau>1 \<rightarrow> \<tau>2)"
@@ -56,12 +58,16 @@ inductive Tm :: "\<Gamma> \<Rightarrow> \<Delta> \<Rightarrow> term \<Rightarrow
 
 | Tm_Let: "\<lbrakk> \<Gamma> , \<Delta> \<turnstile> e1 : \<tau>1 ; BVar x \<tau>1 # \<Gamma> , \<Delta> \<turnstile> e2 : \<tau>2 \<rbrakk> \<Longrightarrow> \<Gamma> , \<Delta> \<turnstile> Let x \<tau>1 e1 e2 : \<tau>2"
 
-| Tm_Case: "\<lbrakk> \<Gamma> , \<Delta> \<turnstile> e : \<tau>1 ; head_data \<tau>1 = Some (T, \<sigma>s) ; \<Gamma> , \<Delta> \<turnstile>\<^sub>t\<^sub>y \<tau> : \<star> ; exhaustive alts \<Delta> T ;
-            \<forall>e |\<in>| set_alts alts. (\<exists>K tys vals e' cty ks.
-                e = MatchCtor K tys vals e' \<and>
-                AxCtor K cty \<in> set \<Delta> \<and> ctor_type cty = Some (T, ks) \<and>
-                \<Gamma> , \<Delta> \<turnstile> e' : \<tau>
-              ) \<rbrakk> \<Longrightarrow> \<Gamma> , \<Delta> \<turnstile> Case e alts : \<tau>"
+| Tm_Case: "\<lbrakk> \<Gamma> , \<Delta> \<turnstile> e : \<tau>1 ; head_data \<tau>1 = Some (T, \<sigma>s) ; \<Gamma> , \<Delta> \<turnstile>\<^sub>t\<^sub>y \<tau> : \<star> ; exhaustive alts \<Delta> T ; Alts \<Gamma> \<Delta> e alts \<tau> \<rbrakk> \<Longrightarrow> \<Gamma> , \<Delta> \<turnstile> Case e alts : \<tau>"
+
+| Alts_Nil: "Alts \<Gamma> \<Delta> e ANil \<tau>"
+
+| Alts_Cons: "\<lbrakk> Alt \<Gamma> \<Delta> e alt \<tau> ; Alts \<Gamma> \<Delta> e alts \<tau> \<rbrakk> \<Longrightarrow> Alts \<Gamma> \<Delta> e (ACons alt alts) \<tau>"
+
+| Alt_Ctor: "\<lbrakk> \<Gamma> , \<Delta> \<turnstile> e : \<tau>1 ; head_data \<tau>1 = Some (T, \<sigma>s) ; \<Gamma> , \<Delta> \<turnstile>\<^sub>t\<^sub>y \<tau> : \<star> ;
+               AxCtor K cty \<in> set \<Delta> ; ctor_type cty = Some (T, ks) ; subst_ctor cty \<sigma>s = Some args ;
+               length vals = length args ; length tys = length ks ;
+               zip_with BVar vals args @ zip_with BTyVar tys ks @ \<Gamma> , \<Delta> \<turnstile> e' : \<tau> \<rbrakk> \<Longrightarrow> Alt \<Gamma> \<Delta> e (MatchCtor K tys vals e') \<tau>"
 
 equivariance Tm
 
@@ -88,6 +94,10 @@ inductive_cases TmE[elim!]:
   "\<Gamma> , \<Delta> \<turnstile> App e1 e2 : \<tau>2"
   "\<Gamma> , \<Delta> \<turnstile> TApp e \<tau> : \<tau>2"
   "\<Gamma> , \<Delta> \<turnstile> Ctor D : \<tau>"
+  "\<Gamma> , \<Delta> \<turnstile> Case e alts : \<tau>"
+
+inductive_cases AltsE[elim!]:
+  "Alts \<Gamma> \<Delta> e (ACons alt alts) \<tau>"
 
 (* Split induction principles *)
 lemma Ty_induct[consumes 1, case_names Var App Data Arrow Forall]:
@@ -111,9 +121,9 @@ lemma Tm_induct[consumes 1, case_names Var Abs App TAbs TApp Ctor Let Case]:
   and "\<And>\<Gamma> \<Delta> e a k \<sigma> \<tau>. \<lbrakk> \<Gamma> , \<Delta> \<turnstile> e : \<forall> a : k . \<sigma> ; P \<Gamma> \<Delta> e (\<forall> a : k . \<sigma>) ; \<Gamma> , \<Delta> \<turnstile>\<^sub>t\<^sub>y \<tau> : k \<rbrakk> \<Longrightarrow> P \<Gamma> \<Delta> (TApp e \<tau>) \<sigma>[\<tau>/a]"
   and "\<And>\<Delta> \<Gamma> D \<tau>. \<lbrakk> \<Delta> \<turnstile> \<Gamma> ; AxCtor D \<tau> \<in> set \<Delta> \<rbrakk> \<Longrightarrow> P \<Gamma> \<Delta> (Ctor D) \<tau>"
   and "\<And>\<Gamma> \<Delta> e1 \<tau>1 x e2 \<tau>2. \<lbrakk> \<Gamma> , \<Delta> \<turnstile> e1 : \<tau>1 ; P \<Gamma> \<Delta> e1 \<tau>1 ; BVar x \<tau>1 # \<Gamma> , \<Delta> \<turnstile> e2 : \<tau>2 ; P (BVar x \<tau>1 # \<Gamma>) \<Delta> e2 \<tau>2 \<rbrakk> \<Longrightarrow> P \<Gamma> \<Delta> (Let x \<tau>1 e1 e2) \<tau>2"
-  and "\<And>\<Gamma> \<Delta> e \<tau>1 T \<sigma>s \<tau> alts. \<lbrakk> \<Gamma> , \<Delta> \<turnstile> e : \<tau>1 ; P \<Gamma> \<Delta> e \<tau>1 ; head_data \<tau>1 = Some (T, \<sigma>s) ; \<Gamma> , \<Delta> \<turnstile>\<^sub>t\<^sub>y \<tau> : \<star> ; exhaustive alts \<Delta> T ; Alts \<Gamma> \<Delta> T \<sigma>s \<tau>1 alts \<tau> \<rbrakk> \<Longrightarrow> P \<Gamma> \<Delta> (Case e alts) \<tau>"
+  and "\<And>\<Gamma> \<Delta> e \<tau>1 T \<sigma>s \<tau> alts. \<lbrakk> \<Gamma> , \<Delta> \<turnstile> e : \<tau>1 ; P \<Gamma> \<Delta> e \<tau>1 ; head_data \<tau>1 = Some (T, \<sigma>s) ; \<Gamma> , \<Delta> \<turnstile>\<^sub>t\<^sub>y \<tau> : \<star> ; exhaustive alts \<Delta> T ; Alts \<Gamma> \<Delta> e alts \<tau> \<rbrakk> \<Longrightarrow> P \<Gamma> \<Delta> (Case e alts) \<tau>"
 shows "P \<Gamma> \<Delta> e \<tau>"
-  using Tm_Alts.inducts(1)[OF assms(1), of _ "\<lambda>_ _ _ _ _ _ _. True"] assms(2-9) by auto
+  using Tm_Alts_Alt.inducts(1)[OF assms(1), of _ "\<lambda>_ _ _ _ _. True" "\<lambda>_ _ _ _ _. True"] assms(2-9) by auto
 
 (* axiom validity *)
 lemma axioms_valid_aux:
@@ -201,33 +211,41 @@ lemma context_valid_tm: "\<Gamma> , \<Delta> \<turnstile> e : \<tau> \<Longright
   by (induction \<Gamma> \<Delta> e \<tau> rule: Tm_induct) (auto simp: context_valid_ty)
 lemmas context_valid = context_valid_ty context_valid_tm
 
-
-
-(* \<lbrakk> \<Gamma> \<turnstile> e : t ; atom x \<sharp> \<Gamma> \<rbrakk> \<Longrightarrow> atom x \<sharp> e *)
-lemma fresh_in_context_ty: "\<lbrakk> \<Gamma> , \<Delta> \<turnstile>\<^sub>t\<^sub>y \<tau> : k ; atom (a::tyvar) \<sharp> \<Gamma> \<rbrakk> \<Longrightarrow> atom a \<sharp> \<tau>"
+lemma supp_in_context_ty: "\<Gamma> , \<Delta> \<turnstile>\<^sub>t\<^sub>y \<tau> : k \<Longrightarrow> supp \<tau> \<subseteq> supp \<Gamma>"
 proof (induction \<Gamma> \<Delta> \<tau> k rule: Ty_induct)
   case (Var \<Gamma> \<Delta> a k)
-  then show ?case using fresh_at_base(2) fresh_not_isin_tyvar by fastforce
-qed (auto simp: fresh_Cons)
+  then show ?case by (metis \<tau>.supp(1) fresh_def fresh_not_isin_tyvar singletonD subsetCI supp_at_base)
+next
+  case (Forall \<Gamma> \<Delta> a k \<sigma>)
+  from Forall(2) show ?case unfolding supp_Cons binder.supp(2) \<tau>.supp(5) pure_supp supp_at_base by auto
+qed (auto simp: \<tau>.supp pure_supp)
 
-lemma fresh_in_axioms: "\<turnstile> \<Delta> \<Longrightarrow> atom (a::tyvar) \<sharp> \<Delta>"
-proof -
-  fix \<Gamma> \<tau> k
-  assume a: "\<turnstile> \<Delta>"
-  let ?Q = "\<lambda>b c d e. atom a \<sharp> c"
-  let ?W = "\<lambda>b c. atom a \<sharp> b"
+corollary fresh_in_context_ty: "\<lbrakk> \<Gamma> , \<Delta> \<turnstile>\<^sub>t\<^sub>y \<tau> : k ; atom (a::tyvar) \<sharp> \<Gamma> \<rbrakk> \<Longrightarrow> atom a \<sharp> \<tau>"
+  unfolding fresh_def using supp_in_context_ty by blast
 
-  have "(\<turnstile> \<Delta> \<longrightarrow> atom a \<sharp> \<Delta>) \<and> (\<Delta> \<turnstile> \<Gamma> \<longrightarrow> ?W \<Delta> \<Gamma>) \<and> (\<Gamma> , \<Delta> \<turnstile>\<^sub>t\<^sub>y \<tau> : k \<longrightarrow> ?Q \<Gamma> \<Delta> \<tau> k)"
-  proof (induction rule: Ax_Ctx_Ty.induct[of "\<lambda>x. atom a \<sharp> x" ?Q ?W])
-    case (Ax_Ctor \<Delta> \<tau> D)
-    then show ?case using fresh_in_context_ty[OF Ax_Ctor(1) fresh_Nil] fresh_Cons fresh_Nil by fastforce
-  qed (auto simp: fresh_Nil fresh_Cons)
+lemma axioms_cons_valid[elim]: "\<turnstile> ax # \<Delta> \<Longrightarrow> (\<turnstile> \<Delta> \<Longrightarrow> P) \<Longrightarrow> P"
+  by (cases rule: Ax.cases) (auto simp: axioms_valid(2))
 
-  then show ?thesis using a by simp
-qed
+lemma axioms_empty_supp: "\<turnstile> \<Delta> \<Longrightarrow> supp \<Delta> = {}"
+proof (induction \<Delta>)
+  case (Cons a \<Delta>)
+  then show ?case
+  proof (cases a rule: axiom.exhaust)
+    case (AxData D k)
+    then show ?thesis by (metis AxE(1) Cons.IH Cons.prems axiom.supp(1) pure_supp supp_Cons)
+  next
+    case (AxCtor K \<tau>)
+    then have "[] , \<Delta> \<turnstile>\<^sub>t\<^sub>y \<tau> : \<star>" using Cons by blast
+    then have 1: "supp \<tau> = {}" using supp_in_context_ty supp_Nil by blast
+    have 2: "supp \<Delta> = {}" using Cons by auto
+    then show ?thesis using 1 AxCtor axiom.supp(2) pure_supp unfolding supp_Cons by blast
+  qed
+qed (simp add: supp_Nil)
 
-lemma perm_axioms_tyvars[simp]: "\<turnstile> \<Delta> \<Longrightarrow> ((a::tyvar) \<leftrightarrow> b) \<bullet> \<Delta> = \<Delta>"
-  using flip_fresh_fresh fresh_in_axioms by blast
+corollary fresh_in_axioms: "\<turnstile> \<Delta> \<Longrightarrow> atom (a::tyvar) \<sharp> \<Delta>"
+  unfolding fresh_def using axioms_empty_supp by simp
+corollary permute_axioms[simp]: "\<turnstile> \<Delta> \<Longrightarrow> p \<bullet> \<Delta> = \<Delta>"
+  using axioms_empty_supp by (simp add: fresh_star_def supp_perm_eq)
 
 nominal_inductive Ax avoids
   Ty_Forall: a
@@ -241,71 +259,500 @@ proof goal_cases
   then show ?case using 2 fresh_star_def by fastforce
 qed auto
 
+lemma var_strengthen_aux:
+  shows "\<Delta> \<turnstile> \<Gamma>' @ BVar x \<tau> # \<Gamma> \<longrightarrow> \<Delta> \<turnstile> \<Gamma>' @ \<Gamma>"
+  and "\<Gamma>' @ BVar x \<tau> # \<Gamma> , \<Delta> \<turnstile>\<^sub>t\<^sub>y \<sigma> : k \<longrightarrow> \<Gamma>' @ \<Gamma> , \<Delta> \<turnstile>\<^sub>t\<^sub>y \<sigma> : k"
+proof (induction rule: Ctx_Ty_induct_split)
+  case Ctx_Empty
+  then show ?case using context_valid(1) by auto
+next
+  case (Ctx_TyVar \<Gamma>' b k2)
+  then show ?case by (metis Ctx.simps append_Cons fresh_Cons fresh_append)
+next
+  case (Ctx_Var \<Gamma>' \<tau> x)
+  then have "atom x \<sharp> \<Gamma>' @ \<Gamma>" using fresh_append fresh_Cons by blast
+  then show ?case using Ctx_intros(3)[OF Ctx_Var(2)] by simp
+next
+  case (Ty_Var \<Gamma>' b k2)
+  then have "BTyVar b k2 \<in> (\<Gamma>' @ \<Gamma>)" using strengthen_isin_tyvar by simp
+  then show ?case by (rule Ty_intros(1)[OF Ty_Var(2)])
+qed (auto intro: Ty_intros)
+lemma var_strengthen_context: "\<Delta> \<turnstile> \<Gamma>' @ BVar x \<tau> # \<Gamma> \<Longrightarrow> \<Delta> \<turnstile> \<Gamma>' @ \<Gamma>"
+  using var_strengthen_aux by simp
+lemma var_strengthen_ty: "\<Gamma>' @ BVar x \<tau> # \<Gamma> , \<Delta> \<turnstile>\<^sub>t\<^sub>y \<sigma> : k \<Longrightarrow> \<Gamma>' @ \<Gamma> , \<Delta> \<turnstile>\<^sub>t\<^sub>y \<sigma> : k"
+  using var_strengthen_aux by simp
+lemmas strengthen = var_strengthen_context var_strengthen_ty
 
+lemma context_cons_valid[elim]: "(\<Delta>::\<Delta>) \<turnstile> bndr # \<Gamma> \<Longrightarrow> (\<Delta> \<turnstile> \<Gamma> \<Longrightarrow> P) \<Longrightarrow> P"
+  by (cases rule: Ctx.cases) (auto simp: context_valid(1))
 
+lemma isin_subset:
+  fixes \<Gamma>::"\<Gamma>"
+  assumes "\<Delta> \<turnstile> \<Gamma>' @ \<Gamma>"
+  shows "bndr \<in> \<Gamma> \<longrightarrow> bndr \<in> (\<Gamma>' @ \<Gamma>)"
+proof
+  assume "bndr \<in> \<Gamma>"
+  then show "bndr \<in> (\<Gamma>' @ \<Gamma>)"
+  using assms proof (induction \<Gamma>' arbitrary: \<Gamma>)
+    case (Cons b \<Gamma>2)
+    have 1: "\<Delta> \<turnstile> \<Gamma>2 @ \<Gamma>" using Cons(3) by auto
+    have 2: "bndr \<in> (\<Gamma>2 @ \<Gamma>)" by (rule Cons(1)[OF Cons(2) 1])
+    show ?case
+    proof (cases b rule: binder.exhaust)
+      case (BVar x \<tau>)
+      then have "atom x \<sharp> (\<Gamma>2 @ \<Gamma>)" using Cons by auto
+      then show ?thesis using 2 BVar fresh_not_isin_var by (cases bndr rule: binder.exhaust) auto
+    next
+      case (BTyVar a k)
+      then have "atom a \<sharp> (\<Gamma>2 @ \<Gamma>)" using Cons by auto
+      then show ?thesis using 2 BTyVar fresh_not_isin_tyvar by (cases bndr rule: binder.exhaust) auto
+    qed
+  qed auto
+qed
 
+lemma Ty_Forall_Inv:
+  assumes a: "\<Gamma> , \<Delta> \<turnstile>\<^sub>t\<^sub>y (\<forall>a:k. \<sigma>) : \<tau>" and b: "atom a \<sharp> \<Gamma>"
+  shows "BTyVar a k # \<Gamma> , \<Delta> \<turnstile>\<^sub>t\<^sub>y \<sigma> : \<star> \<and> \<tau> = \<star>"
+proof (cases rule: Ty.cases[OF a])
+  case (5 a' k' \<Gamma>' \<Delta>' \<sigma>')
+  then have 1: "(BTyVar a' k # \<Gamma>) , \<Delta> \<turnstile>\<^sub>t\<^sub>y \<sigma>' : \<star>" by simp
+  have valid: "\<turnstile> \<Delta>" by (rule axioms_valid(2)[OF 1])
+  have "(a' \<leftrightarrow> a) \<bullet> \<sigma>' = \<sigma>" using Abs_rename_body[of a' \<sigma>' a \<sigma>] 5(3) by auto
+  then have 2: "((a' \<leftrightarrow> a) \<bullet> (BTyVar a' k # \<Gamma>)) , \<Delta> \<turnstile>\<^sub>t\<^sub>y \<sigma> : \<star>" using Ty.eqvt[OF 1, of "(a' \<leftrightarrow> a)"] valid by auto
+  have 3: "((a' \<leftrightarrow> a) \<bullet> (BTyVar a' k # \<Gamma>)) = BTyVar a k # ((a' \<leftrightarrow> a) \<bullet> \<Gamma>)" using Cons_eqvt flip_fresh_fresh by force
+  have 4: "(a' \<leftrightarrow> a) \<bullet> \<Gamma> = \<Gamma>" by (metis 5(1,5) CtxE(1) b context_valid_ty flip_def swap_fresh_fresh)
+  show ?thesis using 2 3 4 5(4) by argo
+qed simp_all
 
+lemma weaken_isin: "\<lbrakk> bndr \<in> (\<Gamma> @ \<Gamma>') ; \<Delta> \<turnstile> \<Gamma> @ xs @ \<Gamma>' \<rbrakk> \<Longrightarrow> bndr \<in> (\<Gamma> @ xs @ \<Gamma>')"
+proof (induction \<Gamma> arbitrary: bndr \<Gamma>' xs)
+  case Nil
+  then show ?case by (cases bndr rule: binder.exhaust) (auto simp: isin_subset)
+next
+  case (Cons b \<Gamma>)
+  have 1: "\<Delta> \<turnstile> \<Gamma> @ xs @ \<Gamma>'" using Cons(3) Ctx.cases by auto
+  then show ?case
+  proof (cases b rule: binder.exhaust)
+    case (BVar x \<tau>)
+    then show ?thesis using 1 Cons by (cases bndr rule: binder.exhaust) auto
+  next
+    case (BTyVar a k)
+    then show ?thesis using 1 Cons by (cases bndr rule: binder.exhaust) auto
+  qed
+qed
 
-lemma fresh_in_context_term_var:
-  assumes "atom (x::var) \<sharp> \<Gamma>"
-  shows "\<Gamma> , \<Delta> \<turnstile> e : \<tau> \<longrightarrow> atom x \<sharp> e"
-  and "Alts \<Gamma> \<Delta> T \<sigma>s \<tau>1 alts \<tau> \<longrightarrow> atom x \<sharp> alts"
-  and "Alt \<Gamma> \<Delta> T \<sigma> \<tau>1 alt \<tau> \<longrightarrow> atom x \<sharp> alt"
-proof (induction \<Gamma> \<Delta> e \<tau> and \<Gamma> \<Delta> T \<sigma>s \<tau>1 alts \<tau> and rule: Tm_Alts.induct)
+lemma weaken_ty: "\<lbrakk> \<Gamma> @ \<Gamma>' , \<Delta>  \<turnstile>\<^sub>t\<^sub>y \<tau> : k ; \<Delta> \<turnstile> \<Gamma> @ xs @ \<Gamma>' \<rbrakk> \<Longrightarrow> \<Gamma> @ xs @ \<Gamma>' , \<Delta> \<turnstile>\<^sub>t\<^sub>y \<tau> : k"
+proof (nominal_induct \<tau> avoiding: \<Gamma> \<Gamma>' xs k rule: \<tau>.strong_induct)
+  case (TyVar x)
+  have 1: "BTyVar x k \<in> (\<Gamma> @ \<Gamma>')" by (cases rule: Ty.cases[OF TyVar(1)]) auto
+  show ?case by (rule Ty_Var[OF TyVar(2) weaken_isin[OF 1 TyVar(2)]])
+next
+  case (TyData T)
+  then have "AxData T k \<in> set \<Delta>" by blast
+  then show ?case by (rule Ty_Data[OF TyData(2)])
+next
+  case TyArrow
+  then have "k = (\<star> \<rightarrow> \<star> \<rightarrow> \<star>)" by blast
+  then show ?case using Ty_Arrow[OF TyArrow(2)] by argo
+next
+  case (TyApp \<tau>1 \<tau>2)
+  then obtain k1 where P: "\<Gamma> @ \<Gamma>' , \<Delta> \<turnstile>\<^sub>t\<^sub>y \<tau>1 : k1 \<rightarrow> k" "\<Gamma> @ \<Gamma>' , \<Delta> \<turnstile>\<^sub>t\<^sub>y \<tau>2 : k1" by blast
+  have 2: "\<Gamma> @ xs @ \<Gamma>' , \<Delta> \<turnstile>\<^sub>t\<^sub>y \<tau>1 : k1 \<rightarrow> k" by (rule TyApp(1)[OF P(1) TyApp(4)])
+  have 3: "\<Gamma> @ xs @ \<Gamma>' , \<Delta> \<turnstile>\<^sub>t\<^sub>y \<tau>2 : k1" by (rule TyApp(2)[OF P(2) TyApp(4)])
+  show ?case by (rule Ty_App[OF 2 3])
+next
+  case (TyForall a k1 \<sigma>)
+  have P: "(BTyVar a k1 # \<Gamma>) @ \<Gamma>' , \<Delta> \<turnstile>\<^sub>t\<^sub>y \<sigma> : \<star>" "k = \<star>" using Ty_Forall_Inv[OF TyForall(6)] TyForall(1,2) fresh_append by auto
+  have 1: "atom a \<sharp> \<Gamma> @ xs @ \<Gamma>'" using TyForall(1-3) fresh_append by blast
+  have 2: "\<Delta> \<turnstile> (BTyVar a k1 # \<Gamma>) @ xs @ \<Gamma>'" using Ctx_TyVar[OF TyForall(7) 1] by simp
+  have 3: "BTyVar a k1 # \<Gamma> @ xs @ \<Gamma>' , \<Delta> \<turnstile>\<^sub>t\<^sub>y \<sigma> : \<star>" using TyForall(5)[OF P(1) 2] by simp
+  show ?case using Ty_Forall[OF 3] P(2) by simp
+qed
 
+lemma weaken_axioms_ty: "\<lbrakk> \<Gamma> , \<Delta>' @ \<Delta> \<turnstile>\<^sub>t\<^sub>y \<tau> : k ; \<Delta>' @ xs @ \<Delta> \<turnstile> \<Gamma> \<rbrakk> \<Longrightarrow> \<Gamma> ,  \<Delta>' @ xs @ \<Delta> \<turnstile>\<^sub>t\<^sub>y \<tau> : k"
+proof (nominal_induct \<tau> avoiding: \<Delta> \<Delta>' k xs \<Gamma> rule: \<tau>.strong_induct)
+  case (TyApp \<tau>1 \<tau>2)
+  then show ?case using Ty_App by blast
+next
+  case (TyForall a k1 \<sigma>)
+  have P: "BTyVar a k1 # \<Gamma> , \<Delta>' @ \<Delta> \<turnstile>\<^sub>t\<^sub>y \<sigma> : \<star>" "k = \<star>" using Ty_Forall_Inv[OF TyForall(7,5)] by auto
+  have 1: "BTyVar a k1 # \<Gamma> , \<Delta>' @ xs @ \<Delta> \<turnstile>\<^sub>t\<^sub>y \<sigma> : \<star>" by (rule TyForall(6)[OF P(1) Ctx_TyVar[OF TyForall(8,5)]])
+  show ?case using Ty_Forall[OF 1] P(2) by argo
+qed (auto intro: Ty_intros)
+lemmas weaken = weaken_isin weaken_ty weaken_axioms_ty
 
+(* inversion rules for abstractions *)
+lemma T_Abs_Inv:
+  assumes a: "\<Gamma> , \<Delta> \<turnstile> (\<lambda>x : \<tau>1 . e) : \<tau>" and b: "atom x \<sharp> \<Gamma>"
+  obtains \<tau>2 where "BVar x \<tau>1 # \<Gamma> , \<Delta> \<turnstile> e : \<tau>2" "\<tau> = arrow_app \<tau>1 \<tau>2"
+proof (cases rule: Tm.cases[OF a])
+  case (2 x' \<tau>1' \<Gamma>' \<Delta>' e' \<tau>2)
+  then have swap: "(x' \<leftrightarrow> x) \<bullet> e' = e" using Abs_rename_body[of x' e' x e] by auto
+  have valid: "\<turnstile> \<Delta>" using axioms_valid(3)[OF 2(5)] 2(2) by simp
+  show ?thesis
+  proof (cases "atom x' = atom x")
+    case True
+    then show ?thesis using 2 swap that by auto
+  next
+    case False
+    then have 1: "atom x \<sharp> BVar x' \<tau>1' # \<Gamma>'" using b by (simp add: 2 fresh_Cons)
+    have 3: "((x' \<leftrightarrow> x) \<bullet> (BVar x' \<tau>1 # \<Gamma>)) , \<Delta> \<turnstile> (x' \<leftrightarrow> x) \<bullet> e' : \<tau>2" using 2 Tm.eqvt[OF 2(5), of "(x' \<leftrightarrow> x)"] by fastforce
+    have "((x' \<leftrightarrow> x) \<bullet> (BVar x' \<tau>1) # ((x' \<leftrightarrow> x) \<bullet> \<Gamma>)) = BVar x \<tau>1 # \<Gamma>"
+      by (metis "1" "2"(1) "2"(5) CtxE(2) binder.perm_simps(1) context_valid_tm flip_at_simps(1) flip_fresh_fresh fresh_Cons perm_\<tau>_vars)
+    then show ?thesis using 1 2 3 swap that by auto
+  qed
+qed simp_all
 
+lemma T_Let_Inv:
+  assumes a: "\<Gamma> , \<Delta> \<turnstile> Let x \<tau>1 e1 e2 : \<tau>" and b: "atom x \<sharp> \<Gamma>"
+  shows "\<Gamma> , \<Delta> \<turnstile> e1 : \<tau>1 \<and> BVar x \<tau>1 # \<Gamma> , \<Delta> \<turnstile> e2 : \<tau>"
+proof (cases rule: Tm.cases[OF a])
+  case (7 \<Gamma>' \<Delta>' e1' \<tau>1' x' e2' \<tau>2')
+  have swap: "(x' \<leftrightarrow> x) \<bullet> e2' = e2" using Abs_rename_body[of x' e2' x e2] 7(3) by simp
+  show ?thesis
+  proof (cases "atom x' = atom x")
+    case True
+    then show ?thesis using 7 swap by auto
+  next
+    case False
+    then have 1: "atom x \<sharp> BVar x' \<tau>1 # \<Gamma>'" using b by (simp add: 7 fresh_Cons)
+    have 2: "((x' \<leftrightarrow> x) \<bullet> (BVar x' \<tau>1#\<Gamma>)) , \<Delta> \<turnstile> (x' \<leftrightarrow> x) \<bullet> e2' : \<tau>" using Tm.eqvt[OF 7(6), of "(x' \<leftrightarrow> x)"] 7 by auto
+    have 3: "((x' \<leftrightarrow> x) \<bullet> (BVar x' \<tau>1) # ((x' \<leftrightarrow> x) \<bullet> \<Gamma>)) = BVar x \<tau>1#\<Gamma>"
+      by (metis "1" 7(1,6) CtxE(2) binder.perm_simps(1) context_valid_tm flip_at_simps(1) flip_def fresh_Cons perm_\<tau>_vars swap_fresh_fresh)
+    from 2 3 7 swap show ?thesis by auto
+  qed
+qed simp_all
 
+lemma T_AbsT_Inv:
+  assumes a: "\<Gamma> , \<Delta> \<turnstile> (\<Lambda> a : k . e) : \<tau>" and b: "atom a \<sharp> \<Gamma>" "atom a \<sharp> \<tau>"
+  obtains \<sigma> where "BTyVar a k # \<Gamma> , \<Delta> \<turnstile> e : \<sigma>" "\<tau> = (\<forall> a:k. \<sigma>)"
+proof (cases rule: Tm.cases[OF a])
+  case (4 a' k' \<Gamma>' \<Delta>' e' \<sigma>')
+  then have fresh: "atom a' \<sharp> \<Gamma>" by (cases rule: Ctx.cases[OF context_valid(2)[OF 4(5)]]) auto
+  have swap: "(a' \<leftrightarrow> a) \<bullet> e' = e" using Abs_rename_body[of a' e' a e] 4(3) by simp
+  have valid: "\<turnstile> \<Delta>" using axioms_valid(3)[OF 4(5)] 4(2) by simp
+  show ?thesis
+  proof (cases "atom a = atom a'")
+    case True
+    then show ?thesis by (metis 4 Abs1_eq_iff(3) atom_eq_iff term_alt_list_alt.eq_iff(6) that)
+  next
+    case False
+    then have 1: "atom a \<sharp> BTyVar a' k # \<Gamma>" using b by (simp add: 4 fresh_Cons)
+    have 2: "((a' \<leftrightarrow> a) \<bullet> (BTyVar a' k # \<Gamma>)), \<Delta> \<turnstile> (a' \<leftrightarrow> a) \<bullet> e' : (a' \<leftrightarrow> a) \<bullet> \<sigma>'" using Tm.eqvt[OF 4(5), of "(a' \<leftrightarrow> a)"] valid 4 by auto
+    have "((a' \<leftrightarrow> a) \<bullet> (BTyVar a' k # \<Gamma>)) = ((a' \<leftrightarrow> a) \<bullet> BTyVar a' k) # \<Gamma>" using 1 fresh flip_fresh_fresh b(1) by simp
+    then have "((a' \<leftrightarrow> a) \<bullet> (BTyVar a' k # \<Gamma>)) = BTyVar a k # \<Gamma>" by (simp add: flip_fresh_fresh)
+    then have "BTyVar a k # \<Gamma> , \<Delta> \<turnstile> e : (a' \<leftrightarrow> a) \<bullet> \<sigma>'" using 2 swap by argo
+    then show ?thesis by (metis "4"(3,4) Abs1_eq_iff(3) False \<tau>.eq_iff(5) \<tau>.fresh(5) b(2) empty_iff flip_commute insert_iff list.set(1,2) term_alt_list_alt.eq_iff(6) that)
+  qed
+qed simp_all
 
+lemma zip_with_context_fresh_vars: "\<lbrakk> \<Delta> \<turnstile> zip_with BVar vars xs @ \<Gamma> ; length vars \<le> length xs \<rbrakk> \<Longrightarrow> set (map atom vars) \<sharp>* \<Gamma>"
+proof (induction vars arbitrary: xs)
+  case Nil
+  then show ?case using fresh_star_def by auto
+next
+  case (Cons a vars)
+  then obtain x xs' where P: "xs = x # xs'" by (cases xs) auto
+  then have 1: "length vars \<le> length xs'" using Cons by simp
+  let ?\<Gamma> = "zip_with BVar vars xs' @ \<Gamma>"
+  from P have "\<Delta> \<turnstile> BVar a x # ?\<Gamma>" using Cons(2) by simp
+  then have "?\<Gamma> , \<Delta> \<turnstile>\<^sub>t\<^sub>y x : \<star>" and 2:"atom a \<sharp> ?\<Gamma>" by auto
+  then have 3: "\<Delta> \<turnstile> ?\<Gamma>" using context_valid(1) by simp
+  show ?case using Cons(1)[OF 3 1] 2 fresh_append
+    by (metis (no_types, lifting) fresh_star_def list.simps(9) set_ConsD)
+qed
 
+lemma zip_with_context_fresh_tyvars: "\<lbrakk> \<Delta> \<turnstile> zip_with BTyVar tys xs @ \<Gamma> ; length tys \<le> length xs \<rbrakk> \<Longrightarrow> set (map atom tys) \<sharp>* \<Gamma>"
+proof (induction tys arbitrary: xs)
+  case Nil
+  then show ?case using fresh_star_def by auto
+next
+  case (Cons a vars)
+  then obtain x xs' where P: "xs = x # xs'" by (cases xs) auto
+  then have 1: "length vars \<le> length xs'" using Cons by simp
+  let ?\<Gamma> = "zip_with BTyVar vars xs' @ \<Gamma>"
+  from P have "\<Delta> \<turnstile> BTyVar a x # ?\<Gamma>" using Cons(2) by simp
+  then have 3: "\<Delta> \<turnstile> ?\<Gamma>" "atom a \<sharp> ?\<Gamma>" by auto
+  show ?case using Cons(1)[OF 3(1) 1] 3(2) fresh_append
+    by (metis (no_types, lifting) fresh_star_def list.simps(9) set_ConsD)
+qed
 
+lemma context_valid_append: "\<Delta>::\<Delta> \<turnstile> \<Gamma>' @ \<Gamma> \<Longrightarrow> \<Delta> \<turnstile> \<Gamma>"
+proof (induction \<Gamma>')
+  case (Cons a \<Gamma>')
+  then show ?case using context_valid(1) by (cases a rule: binder.exhaust) auto
+qed auto
 
+lemma axioms_split_valid: "\<turnstile> \<Delta>' @ \<Delta> \<Longrightarrow> \<turnstile> \<Delta>"
+proof (induction \<Delta>')
+  case (Cons a \<Delta>')
+  then show ?case using axioms_valid(2) by (cases a rule: axiom.exhaust) auto
+qed simp
 
+lemma axioms_regularity: "\<turnstile> \<Delta>' @ AxCtor D \<tau> # \<Delta> \<Longrightarrow> [] , \<Delta> \<turnstile>\<^sub>t\<^sub>y \<tau> : \<star>"
+  using Ax_Ctor axioms_split_valid by (induction \<Delta>) blast+
 
+lemma context_regularity: "\<Delta> \<turnstile> \<Gamma>' @ BVar x \<tau> # \<Gamma> \<Longrightarrow> \<Gamma> , \<Delta> \<turnstile>\<^sub>t\<^sub>y \<tau> : \<star>"
+  using Ctx_Var context_valid_append by (induction \<Gamma>) blast+
 
+lemma isin_same_kind: "\<lbrakk> BTyVar a k1 \<in> (\<Gamma>' @ BTyVar a k2 # \<Gamma>) ; \<Delta> \<turnstile> \<Gamma>' @ BTyVar a k2 # \<Gamma> \<rbrakk> \<Longrightarrow> k1 = k2"
+proof (induction \<Gamma>')
+  case (Cons bndr \<Gamma>')
+  then show ?case by (cases rule: Ctx.cases[OF Cons(3)]) (auto split: if_splits simp: fresh_Cons fresh_append fresh_at_base(2))
+qed auto
 
+lemma isin_same_type: "\<lbrakk> BVar x \<tau> \<in> (\<Gamma>' @ BVar x \<tau>2 # \<Gamma>) ; \<Delta> \<turnstile> \<Gamma>' @ BVar x \<tau>2 # \<Gamma> \<rbrakk> \<Longrightarrow> \<tau> = \<tau>2"
+proof (induction \<Gamma>')
+  case (Cons a \<Gamma>')
+  then show ?case by (cases rule: Ctx.cases[OF Cons(3)]) (auto split: if_splits simp: fresh_Cons fresh_append fresh_at_base)
+qed auto
+lemmas isin_same = isin_same_kind isin_same_type
 
+lemma isin_subst_tyvar: "\<lbrakk> BTyVar a k \<in> (\<Gamma>' @ BTyVar b k2 # \<Gamma>) ; \<Delta> \<turnstile> \<Gamma>' @ BTyVar b k2 # \<Gamma> ; a \<noteq> b \<rbrakk> \<Longrightarrow> BTyVar a k \<in> (\<Gamma>'[\<sigma>/b] @ \<Gamma>)"
+proof (induction \<Gamma>')
+  case (Cons bndr \<Gamma>')
+  then show ?case
+  proof (cases rule: Ctx.cases[OF Cons(3)])
+    case (2 \<Gamma>2 c k3)
+    then have "BTyVar a k = bndr \<or> BTyVar a k \<in> (\<Gamma>' @ BTyVar b k2 # \<Gamma>)" by (metis Cons.prems(1) Cons_eq_append_conv isin.simps(5) list.inject)
+    then show ?thesis
+    proof
+      assume a: "BTyVar a k = bndr"
+      then show ?thesis using 2 Cons by auto
+    next
+      assume "BTyVar a k \<in> (\<Gamma>' @ BTyVar b k2 # \<Gamma>)"
+      then show ?thesis using 2 Cons fresh_not_isin_tyvar by auto
+    qed
+  next
+    case (3 \<Gamma> \<tau> x)
+    then show ?thesis using Cons by auto
+  qed simp
+qed simp
 
+lemma axiom_isin_split: "\<lbrakk> b \<in> set \<Delta> ; \<turnstile> \<Delta> \<rbrakk> \<Longrightarrow> \<exists>\<Delta>1 \<Delta>2. \<Delta> = \<Delta>1 @ b # \<Delta>2"
+proof (induction \<Delta>)
+  case (Cons a \<Delta>)
+  then show ?case
+  proof (cases "a = b")
+    case True
+    then show ?thesis by blast
+  next
+    case False
+    then show ?thesis by (meson Cons.prems(1) split_list)
+  qed
+qed simp
 
+lemma type_substitution_aux:
+  assumes "\<Gamma> , \<Delta> \<turnstile>\<^sub>t\<^sub>y \<sigma> : k"
+  shows "(\<Delta> \<turnstile> (\<Gamma>' @ BTyVar a k # \<Gamma>) \<longrightarrow> \<Delta> \<turnstile> (subst_context \<Gamma>' \<sigma> a @ \<Gamma>))"
+    and "(\<Gamma>' @ BTyVar a k # \<Gamma> , \<Delta> \<turnstile>\<^sub>t\<^sub>y \<tau> : k2 \<longrightarrow> subst_context \<Gamma>' \<sigma> a @ \<Gamma> , \<Delta> \<turnstile>\<^sub>t\<^sub>y subst_type \<tau> \<sigma> a : k2)"
+proof (induction rule: Ctx_Ty_induct_split)
+  case Ctx_Empty
+  then show ?case using context_valid(1)[OF assms] by simp
+next
+  case (Ctx_TyVar \<Gamma>' b k2)
+  then have "atom b \<sharp> \<sigma>" using assms fresh_Cons fresh_append fresh_in_context_ty by blast
+  then have 1: "atom b \<sharp> \<Gamma>'[\<sigma>/a] @ \<Gamma>" by (meson Ctx_TyVar(3) fresh_Cons fresh_append fresh_subst_context_tyvar)
+  show ?case using Ax_Ctx_Ty.Ctx_TyVar[OF Ctx_TyVar(2) 1] assms by auto
+next
+  case (Ctx_Var \<Gamma>' \<tau> x)
+  have 1: "atom x \<sharp> \<Gamma>'[\<sigma>/a] @ \<Gamma>" by (meson Ctx_Var(3) fresh_Cons fresh_append fresh_subst_context_var)
+  show ?case using Ax_Ctx_Ty.Ctx_Var[OF Ctx_Var(2) 1] by simp
+next
+  case (Ty_Var \<Gamma>' b k2)
+  then show ?case
+    proof (cases "b = a")
+    case True
+    then have "k = k2" using isin_same(1) Ty_Var by blast
+    then have "\<Gamma> , \<Delta> \<turnstile>\<^sub>t\<^sub>y (TyVar b)[\<sigma>/a] : k2" using True assms(1) by simp
+    then show ?thesis using weaken_ty[of "[]"] Ty_Var(2) by auto
+  next
+    case False
+    have 1: "BTyVar b k2 \<in> (\<Gamma>'[\<sigma>/a] @ \<Gamma>)" by (rule isin_subst_tyvar[OF Ty_Var(3,1) False])
+    show ?thesis using Ax_Ctx_Ty.Ty_Var[OF Ty_Var(2) 1] False by simp
+  qed
+next
+  case (Ty_Forall \<Gamma>' b k2 \<sigma>')
+  have 1: "a \<noteq> b" by (metis CtxE(1) Ty_Forall(1) binder.fresh(2) context_valid_ty fresh_Cons fresh_append fresh_at_base(2))
+  then have 2: "BTyVar b k2 # \<Gamma>'[\<sigma>/a] @ \<Gamma> , \<Delta> \<turnstile>\<^sub>t\<^sub>y \<sigma>'[\<sigma>/a] : \<star>" using Ty_Forall(2) by simp
+  show "\<Gamma>'[\<sigma>/a] @ \<Gamma> , \<Delta> \<turnstile>\<^sub>t\<^sub>y (\<forall> b : k2 . \<sigma>')[\<sigma>/a] : \<star>" using Ax_Ctx_Ty.Ty_Forall[OF 2]
+    by (metis "1" "2" CtxE(1) assms atom_eq_iff context_valid_ty fresh_Pair fresh_append fresh_at_base(2) fresh_in_context_ty subst_type.simps(5))
+qed (auto intro: Ty_intros)
+corollary type_substitution_context: "\<lbrakk> \<Delta> \<turnstile> \<Gamma>' @ BTyVar a k # \<Gamma> ; \<Gamma> , \<Delta> \<turnstile>\<^sub>t\<^sub>y \<sigma> : k \<rbrakk> \<Longrightarrow> \<Delta> \<turnstile> \<Gamma>'[\<sigma>/a] @ \<Gamma>"
+  using type_substitution_aux by blast
+corollary type_substitution_ty: "\<lbrakk> \<Gamma>' @ BTyVar a k # \<Gamma> , \<Delta> \<turnstile>\<^sub>t\<^sub>y \<tau> : k2 ; \<Gamma> , \<Delta> \<turnstile>\<^sub>t\<^sub>y \<sigma> : k \<rbrakk> \<Longrightarrow> \<Gamma>'[\<sigma>/a] @ \<Gamma> , \<Delta> \<turnstile>\<^sub>t\<^sub>y \<tau>[\<sigma>/a] : k2"
+  using type_substitution_aux by blast
 
-
-
-
-thm Tm_Alts.induct[of "\<lambda>_ _ e _. atom x \<sharp> e" "\<lambda>_ _ _ _ _ alts _. atom x \<sharp> alts" \<Gamma> \<Delta> e \<tau> \<Gamma> \<Delta> T \<sigma> \<tau>1 alts \<tau>]
-
-
-
-lemma fresh_in_context_term_var: "\<lbrakk> \<Gamma> , \<Delta> \<turnstile> e : \<tau> ; atom (x::var) \<sharp> \<Gamma> \<rbrakk> \<Longrightarrow> atom x \<sharp> e"
+lemma typing_regularity: "\<Gamma> , \<Delta> \<turnstile> e : \<tau> \<Longrightarrow> \<Gamma> , \<Delta> \<turnstile>\<^sub>t\<^sub>y \<tau> : \<star>"
 proof (induction \<Gamma> \<Delta> e \<tau> rule: Tm_induct)
   case (Var \<Gamma> \<Delta> x \<tau>)
-  then show ?case using fresh_ineq_at_base fresh_not_isin_var by force
+  then obtain \<Gamma>1 \<Gamma>2 where 1: "\<Gamma> = \<Gamma>1 @ BVar x \<tau> # \<Gamma>2" using isin_split by blast
+  then have "\<Gamma>2 , \<Delta> \<turnstile>\<^sub>t\<^sub>y \<tau> : \<star>" using context_regularity Var(1) by blast
+  then show ?case using weaken_ty[of "[]" \<Gamma>2 \<Delta> \<tau> \<star> "\<Gamma>1 @ [BVar x \<tau>]"] Var(1) 1 by simp
 next
-  case (Case \<Gamma> \<Delta> e \<tau>1 T \<sigma>s \<tau> alts)
-  then show ?case sorry
-qed (auto simp: fresh_Cons)
+  case (Abs x \<tau>1 \<Gamma> \<Delta> e \<tau>2)
+  have 1: "\<Gamma> , \<Delta> \<turnstile>\<^sub>t\<^sub>y \<tau>1 : \<star>" using context_regularity context_valid(1)[OF Abs(2)] by blast
+  have 2: "\<Gamma> , \<Delta> \<turnstile>\<^sub>t\<^sub>y \<tau>2 : \<star>" using strengthen(2)[of "[]"] Abs(2) by force
+  have 3: "\<Delta> \<turnstile> \<Gamma>" by (rule context_valid(1)[OF 1])
+  show ?case by (rule Ty_App[OF Ty_App[OF Ty_Arrow[OF 3] 1] 2])
+next
+  case (TApp \<Gamma> \<Delta> e a k \<sigma> \<tau>)
+  obtain a' \<sigma>' where P: "(\<forall> a:k. \<sigma>) = (\<forall> a':k. \<sigma>')" "BTyVar a' k # \<Gamma> , \<Delta> \<turnstile>\<^sub>t\<^sub>y \<sigma>' : \<star>" by (cases rule: Ty.cases[OF TApp(3)]) auto
+  have "\<Gamma> , \<Delta> \<turnstile>\<^sub>t\<^sub>y \<sigma>'[\<tau>/a'] : \<star>" using type_substitution_ty[of "[]", OF _ TApp(2)] P by auto
+  then show ?case using P(1) subst_type_same by auto
+next
+  case (Ctor \<Delta> \<Gamma> D \<tau>)
+  from Ctor(1) have 1: "\<turnstile> \<Delta>" by (rule axioms_valid(1))
+  then obtain \<Delta>1 \<Delta>2 where 2: "\<Delta> = \<Delta>1 @ AxCtor D \<tau> # \<Delta>2" using axiom_isin_split[OF Ctor(2) 1] by blast
+  then have "[] , \<Delta>2 \<turnstile>\<^sub>t\<^sub>y \<tau> : \<star>" using axioms_regularity 1 by blast
+  then have "[] , \<Delta> \<turnstile>\<^sub>t\<^sub>y \<tau> : \<star>" using weaken(3)[of "[]" "[]" \<Delta>2 \<tau> \<star> "\<Delta>1 @ [AxCtor D \<tau>]"] 1 2 Ctx_Empty by simp
+  then show ?case using weaken(2)[of "[]" "[]"] Ctor(1) by simp
+next
+  case (Let \<Gamma> e1 \<tau>1 x e2 \<tau>2)
+  then show ?case using strengthen(2)[of "[]"] by force
+qed (auto intro: Ty_intros)
 
-lemma fresh_in_context_term_tyvar: "\<lbrakk> \<Gamma> , \<Delta> \<turnstile> e : \<tau> ; atom (a::tyvar) \<sharp> \<Gamma> \<rbrakk> \<Longrightarrow> atom a \<sharp> e"
-proof (induction \<Gamma> \<Delta> e \<tau> rule: Tm.induct)
-  case (Tm_Abs x \<tau>1 \<Gamma> \<Delta> e \<tau>2)
-  then have "atom a \<sharp> \<tau>1" by (meson CtxE(2) context_valid_tm fresh_in_context_ty)
-  then show ?case by (simp add: Tm_Abs fresh_Cons)
+corollary supp_cty: "\<lbrakk> \<turnstile> \<Delta> ; AxCtor K cty \<in> set \<Delta> \<rbrakk> \<Longrightarrow> supp cty = {}"
+  using axioms_empty_supp by (metis axiom.supp(2) axioms_split_valid split_list sup_bot.neutr_eq_iff supp_Cons) 
+
+lemma supp_args:
+  assumes "\<Gamma> , \<Delta> \<turnstile> e : \<tau>1" "head_data \<tau>1 = Some (T, \<sigma>s)" "AxCtor K cty \<in> set \<Delta>" "subst_ctor cty \<sigma>s = Some args"
+  shows "supp args \<subseteq> supp \<Gamma>"
+proof -
+  have 1: "supp cty = {}" by (rule supp_cty[OF axioms_valid(3)[OF assms(1)] assms(3)])
+  have "\<Gamma> , \<Delta> \<turnstile>\<^sub>t\<^sub>y \<tau>1 : \<star>" by (rule typing_regularity[OF assms(1)])
+  then have "supp \<tau>1 \<subseteq> supp \<Gamma>" by (rule supp_in_context_ty)
+  then have "supp \<sigma>s \<subseteq> supp \<Gamma>" using supp_head_data[OF assms(2)] by simp
+  then show "supp args \<subseteq> supp \<Gamma>" using supp_subst_ctor[OF assms(4)] 1 by simp
+qed
+
+lemma Alt_Ctor_Inv: 
+  assumes a: "Alt \<Gamma> \<Delta> e (MatchCtor K tys vals e') \<tau>"
+  and fresh: "set (map atom tys) \<sharp>* \<Gamma>" "set (map atom vals) \<sharp>* \<Gamma>" "set (map atom tys) \<sharp>* \<tau>"
+obtains \<tau>1 T \<sigma>s cty ks args where "\<Gamma> , \<Delta> \<turnstile> e : \<tau>1" "head_data \<tau>1 = Some (T, \<sigma>s)" "\<Gamma> , \<Delta> \<turnstile>\<^sub>t\<^sub>y \<tau> : \<star>" "AxCtor K cty \<in> set \<Delta>" "ctor_type cty = Some (T, ks)"
+  "length args = length vals" "length ks = length tys"
+  "subst_ctor cty \<sigma>s = Some args" "zip_with BVar vals args @ zip_with BTyVar tys ks @ \<Gamma> , \<Delta> \<turnstile> e' : \<tau>"
+proof (cases rule: Alt.cases[OF a])
+  case (1 \<Gamma>2 \<Delta>2 e2 \<tau>1 T \<sigma>s \<tau>2 K2 cty ks args vals2 tys2 e'2)
+  let ?tys = "map atom tys" and ?vals = "map atom vals"
+  let ?tys2 = "map atom tys2" and ?vals2 = "map atom vals2"
+  from 1 have 2: "[?tys2 @ ?vals2]lst. e'2 = [?tys @ ?vals]lst. e'" by simp
+  from 1 have valid: "\<Delta> \<turnstile> zip_with BVar vals2 args @ zip_with BTyVar tys2 ks @ \<Gamma>" using context_valid(2) by simp
+  then have valid_axioms: "\<turnstile> \<Delta>" by (rule axioms_valid(1))
+
+  have g1: "set ?vals2 \<sharp>* \<Gamma>" using zip_with_context_fresh_vars[OF valid] 1(12) fresh_append by (simp add: fresh_star_list(1))
+  have g2: "set ?tys2 \<sharp>* \<Gamma>" using zip_with_context_fresh_tyvars valid context_valid_append 1(13) by (metis order_refl)
+  then have g: "set (?tys2 @ ?vals2) \<sharp>* \<Gamma>" using g1 using fresh_star_Un by auto 
+
+  obtain p where P: "p \<bullet> e'2 = e'" "p \<bullet> (?tys2 @ ?vals2) = ?tys @ ?vals" "supp p \<subseteq> set (?tys2 @ ?vals2) \<union> set (?tys @ ?vals)" by (rule Abs_rename_body_star[OF 2])
+  have G: "supp \<Gamma> \<inter> supp p = {}" using g fresh(1-2) P(3) unfolding fresh_star_def fresh_def using UnE disjoint_iff set_append subsetD by auto
+  then have 3: "p \<bullet> \<Gamma> = \<Gamma>" by (meson disjoint_iff fresh_def fresh_star_def supp_perm_eq_test) 
+
+  from 1(1,2,5) g have t1: "set (?tys2 @ ?vals2) \<sharp>* \<tau>" using fresh_in_context_ty[OF 1(8)] unfolding fresh_star_def by auto
+  have t2: "set (?tys @ ?vals) \<sharp>* \<tau>" using fresh(3) unfolding fresh_star_def by auto
+  then have "supp \<tau> \<inter> supp p = {}" using t1 P(3) unfolding fresh_star_def fresh_def by blast
+  then have 4: "p \<bullet> \<tau> = \<tau>" by (meson disjoint_iff fresh_def fresh_star_def supp_perm_eq_test) 
+
+  have "supp cty = {}" using supp_cty[OF valid_axioms] 1(2,9) by simp
+  then have 5: "supp args \<subseteq> supp \<sigma>s" using supp_subst_ctor 1(11) by blast
+
+  have "supp args \<subseteq> supp \<Gamma>" using supp_args[OF 1(6,7,9,11)] 1(1) by argo
+  then have "supp args \<inter> supp p = {}" using G by blast
+  then have 6: "p \<bullet> args = args" by (meson disjoint_iff fresh_def fresh_star_def supp_perm_eq)
+  have 7: "p \<bullet> vals2 = vals" "p \<bullet> tys2 = tys" using permute_atoms_split[OF P(2)] by auto
+
+  have "p \<bullet> (zip_with BVar vals2 args @ zip_with BTyVar tys2 ks @ \<Gamma>) , p \<bullet> \<Delta> \<turnstile> e' : p \<bullet> \<tau>" using 1(1,2,5,14) P(1) Tm.eqvt by blast
+  then have "zip_with BVar (p \<bullet> vals2) args @ zip_with BTyVar (p \<bullet> tys2) ks @ \<Gamma> , \<Delta> \<turnstile> e' : \<tau>" using 3 4 permute_axioms[OF valid_axioms] 6 by simp
+  then have "zip_with BVar vals args @ zip_with BTyVar tys ks @ \<Gamma> , \<Delta> \<turnstile> e' : \<tau>" using 7 by simp
+  then show ?thesis using 1 that permute_length[OF 7(1)] permute_length[OF 7(2)] by auto
+qed
+
+corollary supp_in_context_term_type: "\<Gamma> , \<Delta> \<turnstile> e : \<tau> \<Longrightarrow> supp \<tau> \<subseteq> supp \<Gamma>"
+  using typing_regularity supp_in_context_ty by blast
+
+lemma supp_in_context_term_aux:
+  shows "\<Gamma> , \<Delta> \<turnstile> e : \<tau> \<longrightarrow> supp e \<subseteq> supp \<Gamma>"
+  and "\<forall>e. Alts \<Gamma> \<Delta> e alts \<tau> \<longrightarrow> supp alts \<subseteq> supp \<Gamma>"
+  and "\<forall>e. Alt \<Gamma> \<Delta> e alt \<tau> \<longrightarrow> supp alt \<subseteq> supp \<Gamma>"
+proof (nominal_induct e and alts and alt avoiding: \<Gamma> \<Delta> \<tau> rule: term_alt_list_alt.strong_induct)
+  case (Var x)
+  then show ?case by (metis TmE(1) fresh_def fresh_not_isin_var singletonD subsetCI supp_at_base term_alt_list_alt.supp(1))
 next
-  case (Tm_Let \<Gamma> e1 e2 \<tau>1 \<tau>2 x)
-  then show ?case
-    by (metis (mono_tags, lifting) CtxE(2) binder.fresh(1) context_valid_tm fresh_Cons fresh_in_context_ty fresh_ineq_at_base list.set_intros(1) term.fresh(7))
-qed (auto simp: fresh_Cons fresh_in_context_ty)
+  case (App e1 e2)
+  then show ?case by (metis TmE(2) Un_least term_alt_list_alt.supp(2))
+next
+  case (TApp e \<sigma>)
+  then show ?case by (metis TmE(3) Un_least supp_in_context_ty term_alt_list_alt.supp(3))
+next
+  case (Ctor T)
+  then show ?case using term_alt_list_alt.supp(4) pure_supp by auto
+next
+  case (Lam x \<tau>1 e)
+  show ?case
+  proof standard
+    assume a: "\<Gamma> , \<Delta> \<turnstile> \<lambda> x : \<tau>1 . e : \<tau>"
+    then have "\<Gamma> , \<Delta> \<turnstile>\<^sub>t\<^sub>y \<tau>1 : \<star>" by (meson CtxE(2) Lam.hyps(1) T_Abs_Inv context_valid_tm) 
+    then have 1: "supp \<tau>1 \<subseteq> supp \<Gamma>" by (rule supp_in_context_ty)
+    have "supp e \<subseteq> supp (BVar x \<tau>1 # \<Gamma>)" using Lam(4) T_Abs_Inv[OF a Lam(1)] by metis
+    then show "supp (\<lambda> x : \<tau>1 . e) \<subseteq> supp \<Gamma>" unfolding term_alt_list_alt.supp supp_Cons binder.supp supp_at_base using 1 by auto
+  qed
+next
+  case (TyLam a k e)
+  show ?case
+  proof standard
+    assume a: "\<Gamma> , \<Delta> \<turnstile> \<Lambda> a : k . e : \<tau>"
+    have "supp e \<subseteq> supp (BTyVar a k # \<Gamma>)" using TyLam(4) T_AbsT_Inv[OF a TyLam(1,3)] by metis
+    then show "supp (\<Lambda> a : k . e) \<subseteq> supp \<Gamma>" unfolding term_alt_list_alt.supp pure_supp supp_Cons binder.supp supp_at_base by auto
+  qed
+next
+  case (Let x \<tau>1 e1 e2)
+  show ?case
+  proof standard
+    assume a: "\<Gamma> , \<Delta> \<turnstile> Let x \<tau>1 e1 e2 : \<tau>"
+    then have "\<Gamma> , \<Delta> \<turnstile>\<^sub>t\<^sub>y \<tau>1 : \<star>" using Let(1) T_Let_Inv typing_regularity by blast
+    then have 1: "supp \<tau>1 \<subseteq> supp \<Gamma>" by (rule supp_in_context_ty)
+    have "supp e1 \<subseteq> supp \<Gamma>" "supp e2 \<subseteq> supp (BVar x \<tau>1 # \<Gamma>)" using Let(4,5) T_Let_Inv[OF a Let(1)] by blast+
+    then show "supp (Let x \<tau>1 e1 e2) \<subseteq> supp \<Gamma>" unfolding term_alt_list_alt.supp supp_Cons binder.supp supp_at_base using 1 by auto
+  qed
+next
+  case (Case e alts)
+  then show ?case unfolding term_alt_list_alt.supp by blast
+next
+  case ANil
+  then show ?case using term_alt_list_alt.supp by simp
+next
+  case (ACons alt alts)
+  then show ?case unfolding term_alt_list_alt.supp by blast
+next
+  case (MatchCtor K tys vals e')
+  show ?case
+  proof (standard, standard)
+    fix e
+    assume a: "Alt \<Gamma> \<Delta> e (MatchCtor K tys vals e') \<tau>"
+    obtain \<tau>1 T \<sigma>s cty ks args where P: "\<Gamma> , \<Delta> \<turnstile> e : \<tau>1" "head_data \<tau>1 = Some (T, \<sigma>s)" "\<Gamma> , \<Delta> \<turnstile>\<^sub>t\<^sub>y \<tau> : \<star>" "AxCtor K cty \<in> set \<Delta>" "ctor_type cty = Some (T, ks)"
+      "length args = length vals" "length ks = length tys" "subst_ctor cty \<sigma>s = Some args" "zip_with BVar vals args @ zip_with BTyVar tys ks @ \<Gamma> , \<Delta> \<turnstile> e' : \<tau>"
+      by (rule Alt_Ctor_Inv[OF a MatchCtor(1,4,3)])
+    then have "supp e' \<subseteq> supp (zip_with BVar vals args @ zip_with BTyVar tys ks @ \<Gamma>)" using MatchCtor(7) by simp
+    then have "supp e' \<subseteq> supp vals \<union> supp args \<union> supp tys \<union> supp \<Gamma>" unfolding supp_append using supp_zip_with pure_supp by blast
+    then have "supp e' \<subseteq> supp vals \<union> supp tys \<union> supp \<Gamma>" using supp_args[OF P(1,2,4,8)] by blast
+    then show "supp (MatchCtor K tys vals e') \<subseteq> supp \<Gamma>" unfolding term_alt_list_alt.supp pure_supp supp_vars supp_tyvars by auto
+  qed
+qed
+corollary supp_in_context_term: "\<Gamma> , \<Delta> \<turnstile> e : \<tau> \<Longrightarrow> supp e \<union> supp \<tau> \<subseteq> supp \<Gamma>"
+  using supp_in_context_ty[OF typing_regularity] supp_in_context_term_aux(1) by simp
+lemmas supp_in_context = supp_in_context_ty supp_in_context_term
+
+corollary fresh_in_context_term_var: "\<lbrakk> \<Gamma> , \<Delta> \<turnstile> e : \<tau> ; atom (y::var) \<sharp> \<Gamma> \<rbrakk> \<Longrightarrow> atom y \<sharp> e"
+  using supp_in_context_term unfolding fresh_def by blast
+corollary fresh_in_context_term_tyvar: "\<lbrakk> \<Gamma> , \<Delta> \<turnstile> e : \<tau> ; atom (a::tyvar) \<sharp> \<Gamma> \<rbrakk> \<Longrightarrow> atom a \<sharp> e \<and> atom a \<sharp> \<tau>"
+  using supp_in_context_term unfolding fresh_def by blast
 lemmas fresh_in_context = fresh_in_context_ty fresh_in_context_term_var fresh_in_context_term_tyvar
-
-
-
-
-
-
 
 nominal_inductive Tm avoids
   Tm_Abs: x
   | Tm_TAbs: a
   | Tm_Let: x
+  | Alt_Ctor: tys and vals
 proof goal_cases
   case (1 x \<tau>1 \<Gamma> \<Delta> e \<tau>2)
   then have "\<Delta> \<turnstile> BVar x \<tau>1 # \<Gamma>" by (rule context_valid)
@@ -330,6 +777,16 @@ next
   then obtain y e2' where 2: "Let x \<tau>1 e1 e2 = Let y \<tau>1 e1 e2' \<and> atom x \<sharp> Let y \<tau>1 e1 e2'" using Abs_fresh_var by auto
   then have "atom x \<sharp> (\<Gamma>, \<Delta>, Let y \<tau>1 e1 e2', \<tau>2)" using 1 fresh_Pair by simp
   then show ?case using 2 fresh_star_def by fastforce
+next
+  case (7 \<Gamma> \<Delta> e \<tau>1 T \<sigma>s \<tau> K cty ks args vals tys e')
+  have 1: "\<Delta> \<turnstile> zip_with BVar vals args @ zip_with BTyVar tys ks @ \<Gamma>" by (rule context_valid(2)[OF 7(9)])
+  have g1: "set (map atom vals) \<sharp>* \<Gamma>" using zip_with_context_fresh_vars[OF 1] 7(7) unfolding fresh_star_def fresh_append by simp
+  have "set (map atom tys) \<sharp>* \<Gamma>" using zip_with_context_fresh_tyvars[OF context_valid_append[OF 1]] 7(8) by simp
+  then have 2: "(set (map atom vals) \<union> set (map atom tys)) \<sharp>* \<Gamma>" (is "?x \<sharp>* \<Gamma>") using g1 unfolding fresh_star_def by blast
+  have 3: "?x \<sharp>* e" using fresh_in_context(2,3)[OF 7(1)] 2 unfolding fresh_star_def by auto
+  have 4: "?x \<sharp>* \<tau>" using fresh_in_context(1)[OF 7(3)] 2 unfolding fresh_star_def by auto
+  have "?x \<sharp>* \<Delta>" using fresh_in_axioms[OF axioms_valid(3)[OF 7(1)]] unfolding fresh_star_def by auto
+  then show ?case using 2 3 4 unfolding fresh_star_def fresh_Pair by auto
 qed auto
 
 end
